fairness/resources.v
@@ -11,6 +11,7 @@ Class fairnessGpreS (Mdl : FairModel) Λ Σ `{Countable (locale Λ)} := {
   fairnessGpreS_model :> inG Σ (authUR (optionUR (exclR (ModelO Mdl))));
   fairnessGpreS_model_mapping :> inG Σ (authUR (gmapUR (localeO Λ) (exclR (gsetR (RoleO Mdl)))));
   fairnessGpreS_model_fuel :> inG Σ (authUR (gmapUR (RoleO Mdl) (exclR natO)));
+  fairnessGpreS_model_free_roles :> inG Σ (authUR (gset_disjUR (RoleO Mdl)));
 }.
 
 Class fairnessGS (Mdl: FairModel) Λ Σ `{Countable (locale Λ)} := FairnessGS {
@@ -21,17 +22,21 @@ Class fairnessGS (Mdl: FairModel) Λ Σ `{Countable (locale Λ)} := FairnessGS {
   fairness_model_mapping_name : gname;
   (** Mapping of roles to fuel *)
   fairness_model_fuel_name : gname;
+  (** Set of free/availble roles *)
+  fairness_model_free_roles_name : gname;
 }.
 
 Global Arguments FairnessGS Mdl Λ  Σ {_ _ _} _ _ _.
 Global Arguments fairness_model_name {Mdl Λ Σ _ _} _.
 Global Arguments fairness_model_mapping_name {Mdl Λ Σ _ _} _ : assert.
 Global Arguments fairness_model_fuel_name {Mdl Λ Σ _ _} _ : assert.
+Global Arguments fairness_model_free_roles_name {Mdl Λ Σ _ _} _ : assert.
 
 Definition fairnessΣ (Mdl: FairModel) Λ `{Countable (locale Λ)} : gFunctors := #[
    GFunctor (authUR (optionUR (exclR (ModelO Mdl))));
    GFunctor (authUR (gmapUR (localeO Λ) (exclR (gsetR (RoleO Mdl)))));
-   GFunctor (authUR (gmapUR (RoleO Mdl) (exclR natO)))
+   GFunctor (authUR (gmapUR (RoleO Mdl) (exclR natO)));
+   GFunctor (authUR (gset_disjUR (RoleO Mdl)))
 ].
 
 Global Instance subG_fairnessGpreS {Σ Λ Mdl} `{Countable (locale Λ)} :
@@ -159,50 +164,6 @@ Section map_imap.
   Qed.
 End map_imap.
 
-Section locales_utils.
-  Context {Λ: language}.
-
-  Definition locales_of_list_from tp0 (tp: list $ expr Λ): list $ locale Λ :=
-    (λ '(t, e), locale_of t e) <$> (prefixes_from tp0 tp).
-  Notation locales_of_list tp := (locales_of_list_from [] tp).
-
-  Lemma locales_of_list_equiv tp0 tp0' tp1 tp2:
-    locales_equiv_from tp0 tp0' tp1 tp2 →
-    locales_of_list_from tp0 tp1 = locales_of_list_from tp0' tp2.
-  Proof.
-    revert tp0 tp0' tp1. induction tp2; intros tp0 tp0' tp1 H;
-    destruct tp1 as [|e1 tp1]; try by apply Forall2_length in H.
-    unfold locales_of_list_from. simpl.
-    simpl in H. apply Forall2_cons_1 in H as [??]. f_equal =>//.
-    apply IHtp2 =>//.
-  Qed.
-
-  Lemma locales_of_list_step_incl σ1 σ2 oζ tp1 tp2 :
-      locale_step (tp1, σ1) oζ (tp2, σ2) ->
-      locales_of_list tp1 ⊆ locales_of_list tp2.
-  Proof.
-    intros H. inversion H; simplify_eq=>//.
-    replace (t1 ++ e2 :: t2 ++ efs) with ((t1 ++ e2 :: t2) ++ efs); last by list_simplifier.
-    rewrite /locales_of_list_from. rewrite [in X in _ ⊆ X]prefixes_from_app /= fmap_app.
-    assert ((λ '(t, e), locale_of t e) <$> prefixes (t1 ++ e1 :: t2) = (λ '(t, e), locale_of t e) <$> prefixes (t1 ++ e2 :: t2))
-      as ->; last set_solver.
-    apply locales_of_list_equiv, locales_equiv_middle. by eapply locale_step_preserve.
-  Qed.
-
-  Lemma locales_of_list_from_locale_from `{EqDecision (locale Λ)} tp0 tp1 ζ:
-    is_Some (from_locale_from tp0 tp1 ζ) ->
-    ζ ∈ locales_of_list_from tp0 tp1.
-  Proof.
-    revert tp0; induction tp1 as [|e1 tp1 IH]; intros tp0.
-    { simpl. intros H. inversion H. congruence. }
-    simpl. intros [e Hsome]. rewrite /locales_of_list_from /=.
-    destruct (decide (locale_of tp0 e1 = ζ)); simplify_eq; first set_solver.
-    apply elem_of_cons; right. apply IH. eauto.
-  Qed.
-
-End locales_utils.
-Notation locales_of_list tp := (locales_of_list_from [] tp).
-
 Section model_state_interp.
   Context {Mdl: FairModel}.
   Context `{fG: fairnessGS Mdl Λ Σ}.
@@ -235,16 +196,22 @@ Section model_state_interp.
   Definition frag_model_is (M: Mdl): iProp Σ :=
     own (fairness_model_name fG) (◯ Excl' M).
 
+  Definition auth_free_roles_are (FR: gset Role): iProp Σ :=
+    own (fairness_model_free_roles_name fG) (● (GSet FR)).
+
+  Definition frag_free_roles_are (FR: gset Role): iProp Σ :=
+    own (fairness_model_free_roles_name fG) (◯ (GSet FR)).
+
   Definition model_state_interp (tp: list $ expr Λ) (δ: LiveState Mdl): iProp Σ :=
-    ∃ M, auth_fuel_is δ.(ls_fuel) ∗
-      auth_mapping_is M ∗ ⌜maps_inverse_match δ.(ls_mapping) M⌝ ∗
+    ∃ M FR, auth_fuel_is δ.(ls_fuel) ∗ auth_mapping_is M ∗ auth_free_roles_are FR ∗
+      ⌜maps_inverse_match δ.(ls_mapping) M⌝ ∗
       ⌜ ∀ ζ, ζ ∉ locales_of_list tp → M !! ζ = None ⌝ ∗
-      auth_model_is δ.
+      auth_model_is δ ∗ ⌜ FR ∩ dom δ.(ls_fuel) = ∅ ⌝.
 
   Lemma model_state_interp_tids_smaller δ tp :
     model_state_interp tp δ -∗ ⌜ tids_smaller tp δ ⌝.
   Proof.
-    iIntros "(%M&_&_&%Hminv&%Hbig&_)". iPureIntro.
+    iIntros "(%M&%FR&_&_&_&%Hminv&%Hbig&_)". iPureIntro.
     intros ρ ζ Hin.
     assert (¬ (ζ ∉ locales_of_list tp)).
     - intros contra.
@@ -397,6 +364,14 @@ Section adequacy.
     iExists _. by iSplitL "H1".
   Qed.
 
+  Lemma model_free_roles_init `{fairnessGpreS Mdl Λ Σ} (s0: Mdl) (FR: gset _):
+    ⊢ |==> ∃ γ,
+        own (A := authUR (gset_disjUR (RoleO Mdl))) γ (● GSet FR  ⋅ ◯ GSet FR).
+  Proof.
+    iMod (own_alloc (● GSet FR  ⋅ ◯ GSet FR)) as (γ) "[H1 H2]".
+    { apply auth_both_valid_2 =>//. }
+    iExists _. by iSplitL "H1".
+  Qed.
 End adequacy.
 
 Section model_state_lemmas.
@@ -413,6 +388,43 @@ Section model_state_lemmas.
     - iModIntro. iFrame.
   Qed.
 
+  Lemma free_roles_inclusion FR fr:
+    auth_free_roles_are FR -∗
+    frag_free_roles_are fr -∗
+    ⌜fr ⊆ FR⌝.
+  Proof.
+    iIntros "HFR Hfr".
+    iDestruct (own_valid_2 with "HFR Hfr") as %Hval. iPureIntro.
+    apply auth_both_valid_discrete in Hval as [??].
+    by apply gset_disj_included.
+  Qed.
+
+  Lemma update_free_roles rem FR fr1:
+    rem ⊆ fr1 ->
+    auth_free_roles_are FR -∗
+    frag_free_roles_are fr1 ==∗
+    auth_free_roles_are (FR ∖ rem) ∗
+    frag_free_roles_are (fr1 ∖ rem).
+  Proof.
+    iIntros (?) "HFR Hfr1".
+
+    iDestruct (free_roles_inclusion with "HFR Hfr1") as %Hincl.
+
+    replace FR with ((FR ∖ rem) ∪ rem); last first.
+    { rewrite difference_union_L. set_solver. }
+    replace fr1 with ((fr1 ∖ rem) ∪ rem); last first.
+    { rewrite difference_union_L. set_solver. }
+
+    iAssert (frag_free_roles_are (fr1 ∖ rem) ∗ frag_free_roles_are rem)%I with "[Hfr1]" as "[Hfr2 Hrem]".
+    { rewrite /frag_free_roles_are -own_op -auth_frag_op gset_disj_union //. set_solver. }
+
+    iCombine "HFR Hrem" as "H".
+    iMod (own_update with "H") as "[??]" ; eauto.
+    - apply auth_update, gset_disj_dealloc_local_update.
+    - iModIntro. iFrame. iApply (own_proper with "Hfr2").
+      do 2 f_equiv. set_solver.
+  Qed.
+
   Lemma model_agree s1 s2:
     auth_model_is s1 -∗ frag_model_is s2 -∗ ⌜ s1 = s2 ⌝.
   Proof.
@@ -424,7 +436,7 @@ Section model_state_lemmas.
   Lemma model_agree' δ1 s2 n:
     model_state_interp n δ1 -∗ frag_model_is s2 -∗ ⌜ ls_under δ1 = s2 ⌝.
   Proof.
-    iIntros "Hsi Hs2". iDestruct "Hsi" as (?) "(_&_&_&_&Hs1)".
+    iIntros "Hsi Hs2". iDestruct "Hsi" as (??) "(_&_&_&_&_&Hs1&_)".
     iApply (model_agree with "Hs1 Hs2").
   Qed.
 
@@ -450,9 +462,9 @@ Section model_state_lemmas.
        | right _ => F !! ρ
        end) (gset_to_gmap (0%nat) LR).
 
-  Definition update_fuel_resource (δ1: LiveState Mdl) (fs2: gmap (fmrole Mdl) nat) (s2: Mdl):
+  Definition update_fuel_resource (δ1: LiveState Mdl) (fs1 fs2: gmap (fmrole Mdl) nat) (s2: Mdl):
     gmap (fmrole Mdl) nat :=
-    fuel_apply fs2 (δ1.(ls_fuel (Λ := Λ))) (live_roles _ s2).
+    fuel_apply fs2 (δ1.(ls_fuel (Λ := Λ))) (((dom $ ls_fuel δ1) ∪ dom fs2) ∖ (dom fs1 ∖ dom fs2)).
 
   Lemma elem_of_frame_excl_map
         (fs F: gmap (fmrole Mdl) nat)
@@ -666,6 +678,24 @@ Section model_state_lemmas.
   Lemma update_has_fuels_no_step ζ fs fs' F M:
     let LR := (dom F ∪ dom fs') ∖ (dom fs ∖ dom fs') in
     (fs ≠ ∅) ->
+    (dom fs' ⊆ dom fs) ->
+    has_fuels ζ fs -∗
+    auth_fuel_is F -∗
+    auth_mapping_is M ==∗
+      auth_fuel_is (fuel_apply fs' F LR) ∗
+      has_fuels ζ fs' ∗
+      auth_mapping_is (<[ ζ := dom fs' ]> M).
+  Proof.
+    iIntros (LR Hfs Hdom) "Hfuels Hafuels Hamapping".
+    rewrite !has_fuels_equiv. iDestruct "Hfuels" as "[Hmapping Hfuels]".
+    iMod (update_fuel fs fs' with "Hafuels Hfuels") as "[Hafuels Hfuels]"; [done|set_solver|].
+    iMod (update_mapping with "Hamapping Hmapping") as "[Hamapping Hmapping]".
+    iModIntro. iFrame.
+  Qed.
+
+  Lemma update_has_fuels_no_step_no_change ζ fs fs' F M:
+    let LR := (dom F ∪ dom fs') ∖ (dom fs ∖ dom fs') in
+    (fs ≠ ∅) ->
     (dom fs' = dom fs) ->
     has_fuels ζ fs -∗
     auth_fuel_is F -∗
@@ -686,7 +716,7 @@ Section model_state_lemmas.
     has_fuels ζ fs -∗ model_state_interp n δ -∗ ⌜ ∀ ρ, ls_mapping δ !! ρ = Some ζ <-> ρ ∈ dom fs ⌝.
   Proof.
     unfold model_state_interp, has_fuels, auth_mapping_is, frag_mapping_is.
-    iIntros "[Hζ Hfuels] (%M&Hafuel&Hamapping&%Hmapinv&Hamod) %ρ".
+    iIntros "[Hζ Hfuels] (%M&%FR&Hafuel&Hamapping &HFR&%Hmapinv&Hamod&Hfr) %ρ".
     iCombine "Hamapping Hζ" as "H".
     iDestruct (own_valid with "H") as %Hval. iPureIntro.
     apply auth_both_valid_discrete in Hval as [Hval ?].
@@ -703,7 +733,7 @@ Section model_state_lemmas.
     has_fuels ζ fs -∗ model_state_interp n δ -∗  ⌜ ∀ ρ, ρ ∈ dom fs -> ls_fuel δ !! ρ = fs !! ρ ⌝.
   Proof.
     unfold has_fuels, model_state_interp, auth_fuel_is.
-    iIntros "[Hζ Hfuels] (%M&Hafuel&Hamapping&%Hmapinv&Hamod)" (ρ Hρ).
+    iIntros "[Hζ Hfuels] (%M&%FR&Hafuel&Hamapping&HFR&%Hmapinv&Hamod)" (ρ Hρ).
     iDestruct (big_sepS_delete _ _ ρ with "Hfuels") as "[(%f&%Hfs&Hfuel) _]" =>//.
     iCombine "Hafuel Hfuel" as "H".
     iDestruct (own_valid with "H") as %Hval. iPureIntro.
@@ -715,93 +745,159 @@ Section model_state_lemmas.
     rewrite Hfuelρ Hfs //.
   Qed.
 
-  Lemma update_no_step_enough_fuel extr (auxtr : auxiliary_trace (fair_model Mdl)) c2 fs ζ:
+  Lemma update_no_step_enough_fuel extr (auxtr : auxiliary_trace (fair_model Mdl)) rem c2 fs ζ:
     (dom fs ≠ ∅) ->
+    (live_roles _ (trace_last auxtr)) ∩ rem = ∅ →
+    rem ⊆ dom fs →
     locale_step (trace_last extr) (Some ζ) c2 ->
     has_fuels_S ζ fs -∗ model_state_interp (trace_last extr).1 (trace_last auxtr)
     ==∗ ∃ δ2 (ℓ : mlabel $ fair_model Mdl),
         ⌜labels_match (Some ζ) ℓ
         ∧ valid_state_evolution_fairness (extr :tr[Some ζ]: c2) (auxtr :tr[ℓ]: δ2)⌝
-                                ∗ has_fuels ζ fs ∗ model_state_interp c2.1 δ2.
+                                ∗ has_fuels ζ (fs ⇂ (dom fs ∖ rem)) ∗ model_state_interp c2.1 δ2.
   Proof.
-    iIntros "%HnotO %Hstep Hf Hmod".
+    iIntros "%HnotO %Holdroles %Hincl %Hstep Hf Hmod".
     destruct c2 as [tp2 σ2].
     destruct (set_choose_L _ HnotO) as [??].
     iDestruct (has_fuel_in with "Hf Hmod") as %Hxdom; eauto.
     iDestruct (has_fuel_fuel with "Hf Hmod") as "%Hfuel"; eauto.
     iDestruct (model_state_interp_tids_smaller with "Hmod") as %Hζs.
-    iDestruct "Hmod" as "(%M & Hfuel & Hamapping & %Hminv & %Hlocssmall & Hmodel)".
+    iDestruct "Hmod" as "(%M & %FR & Hfuel & Hamapping & HFR & %Hminv & %Hlocssmall & Hmodel & %HFR)".
     unfold has_fuels_S.
     simpl in *.
 
-    iMod (update_has_fuels_no_step ζ (S <$> fs) fs with "[Hf] [Hfuel] [Hamapping]") as "(Hafuels&Hfuels&Hamapping)" =>//.
-    { rewrite -dom_empty_iff_L. set_solver. }
-    { set_solver. }
-    iModIntro.
-    assert (Hfueldom: dom (fuel_apply fs (ls_fuel (trace_last auxtr))
-                                      ((dom (ls_fuel (trace_last auxtr)) ∪ dom fs) ∖ (dom fs ∖ dom fs))) =
-                      live_roles Mdl (trace_last auxtr)).
-    { unfold fuel_apply.
-      assert (dom fs ⊆ live_roles Mdl (trace_last auxtr)).
-      { intros ρ Hin. rewrite -ls_fuel_dom elem_of_dom Hfuel; last set_solver.
+    set new_dom := ((dom (ls_fuel (trace_last auxtr)) ∪ dom fs) ∖ rem).
+    set new_mapping := ls_mapping (trace_last auxtr) ⇂ new_dom.
+
+    assert (dom (fuel_apply (filter (λ '(k, _), k ∈ dom fs ∖ rem) fs) (ls_fuel (trace_last auxtr))
+                   ((dom (ls_fuel (trace_last auxtr)) ∪ dom fs) ∖ rem)) = new_dom) as Hnewdom.
+    { rewrite /fuel_apply map_imap_dom_eq ?dom_gset_to_gmap //.
+      intros ρ0 _ Hindom.
+      destruct (decide (ρ0 ∈ dom (filter (λ '(k, _), k ∈ dom fs ∖ rem) fs))) as [Hinf|Hninf];
+        first by apply elem_of_dom.
+      apply elem_of_difference in Hindom as [Hin1 ?].
+      apply elem_of_union in Hin1 as [?|Hin2]; first by apply elem_of_dom.
+      exfalso. apply Hninf. apply elem_of_dom in Hin2 as [f ?].
+      eapply elem_of_dom_2. rewrite map_filter_lookup_Some. split =>//.
+      apply elem_of_difference; split =>//. by eapply elem_of_dom_2. }
+
+    assert (Hsamedoms: dom new_mapping =
+                       dom (fuel_apply (fs ⇂ (dom fs ∖ rem))
+                                       (ls_fuel (trace_last auxtr))
+                                       ((dom (ls_fuel (trace_last auxtr)) ∪ dom fs) ∖ rem))).
+    { rewrite /new_mapping /new_dom. unfold fuel_apply.
+      assert (dom fs ⊆ dom (trace_last auxtr).(ls_fuel)).
+      { intros ρ Hin. rewrite elem_of_dom Hfuel; last set_solver.
         apply elem_of_dom in Hin as [? Hin]. rewrite lookup_fmap Hin //=. }
-      rewrite (ls_fuel_dom (trace_last auxtr)) map_imap_dom_eq.
-      + rewrite dom_gset_to_gmap. set_solver.
-      + intros ρ _ Hin. rewrite dom_gset_to_gmap in Hin.
-        destruct (decide (ρ ∈ dom fs)) as [Hin'|_].
+      rewrite map_imap_dom_eq; last first.
+      { intros ρ _ Hin. rewrite dom_gset_to_gmap in Hin.
+        destruct (decide (ρ ∈ dom $ fs ⇂ (dom fs ∖ rem))) as [Hin'|_].
         * by apply elem_of_dom.
-        * apply elem_of_dom. rewrite ls_fuel_dom. set_solver. }
-    assert (Hmappingdom: dom (ls_mapping (trace_last auxtr)) = live_roles _ (trace_last auxtr)).
-    { apply ls_mapping_dom. }
+        * apply elem_of_dom. set_solver. }
+      rewrite dom_domain_restrict ?dom_gset_to_gmap ?ls_same_doms //. set_solver. }
+    assert (Hfueldom: live_roles _ (trace_last auxtr) ⊆
+     dom (fuel_apply (fs ⇂ (dom fs ∖ rem))
+                     (ls_fuel (trace_last auxtr))
+                     ((dom (ls_fuel (trace_last auxtr)) ∪ dom fs) ∖ rem))).
+    { rewrite /fuel_apply Hnewdom.
+      intros ρ Hin. apply elem_of_difference; split;
+        [apply ls_fuel_dom in Hin; set_solver | set_solver]. }
+
+    iMod (update_has_fuels_no_step ζ (S <$> fs) (fs ⇂ (dom fs ∖ rem)) with "[Hf] [Hfuel] [Hamapping]") as "(Hafuels&Hfuels&Hamapping)" =>//.
+    { rewrite -dom_empty_iff_L. set_solver. }
+    { rewrite dom_domain_restrict; set_solver. }
+
+    iModIntro.
     iExists {|
       ls_under := (trace_last auxtr).(ls_under);
       ls_fuel := _;
       ls_fuel_dom := Hfueldom;
-      ls_mapping := (trace_last auxtr).(ls_mapping);
-      ls_mapping_dom := Hmappingdom;
+      ls_same_doms := Hsamedoms;
     |}.
     iExists (Silent_step ζ). simpl.
     iSplit; last first.
-    { rewrite (dom_fmap_L _ fs). iFrame "Hfuels". iExists M. rewrite /maps_inverse_match //=. iFrame.
-      iPureIntro. split; first set_solver.
-      unfold tids_smaller; simpl. intros ζ0 Hin.
-      unfold tids_smaller in Hζs.
-      apply Hlocssmall.
-      destruct (trace_last extr).
-      have ? := locales_of_list_step_incl _ _ _ _ _ Hstep. simpl.
-      clear Hfueldom Hmappingdom. set_solver. }
-    iSplit =>//. iSplit; first done. iSplit; last first.
-    { iPureIntro.
-      unfold tids_smaller; simpl. intros ρ ζ0 Hsome.
-      specialize (Hζs _ _ Hsome).
-      destruct (trace_last extr); eapply from_locale_step =>//. }
-    iSplit.
-    { iPureIntro. eexists. apply Hxdom. by rewrite dom_fmap. }
-    iSplit.
-    { unfold fuel_decr. simpl.
-      iIntros "!%" (ρ' Hρ'live Hmustdec).
+    { rewrite (dom_fmap_L _ fs). iFrame "Hfuels". iExists _, FR. rewrite /maps_inverse_match //=. iFrame.
+      assert (dom fs ⊆ dom (ls_fuel $ trace_last auxtr)).
+      { intros ρ Hin. setoid_rewrite dom_fmap in Hxdom.
+        specialize (Hxdom ρ). rewrite -ls_same_doms. apply elem_of_dom. exists ζ.
+        by apply Hxdom. }
+      iSplit.
+      { iApply (auth_fuel_is_proper with "Hafuels"). f_equiv.
+        rewrite dom_domain_restrict; last set_solver.
+        replace (dom fs ∖ (dom fs ∖ rem)) with rem; [set_solver|].
+        rewrite -leibniz_equiv_iff. intros ρ. split; [set_solver|].
+        intros [? [?|?]%not_elem_of_difference]%elem_of_difference =>//. }
+      iPureIntro. split; last split.
+      - intros ρ ζ'. rewrite /new_mapping dom_domain_restrict; last set_solver. split.
+        + intros [Hlk Hin]%map_filter_lookup_Some. destruct (decide (ζ' = ζ)) as [->|Hneq].
+          * rewrite lookup_insert. eexists; split=>//. set_solver.
+          * rewrite lookup_insert_ne //. by apply Hminv.
+        + intros Hin. destruct (decide (ζ' = ζ)) as [->|Hneq].
+          * rewrite lookup_insert in Hin. apply map_filter_lookup_Some.
+            destruct Hin as (?&?&?). simplify_eq. split; last set_solver.
+            apply Hxdom. rewrite dom_fmap. set_solver.
+          * rewrite lookup_insert_ne // -Hminv in Hin. apply map_filter_lookup_Some; split=>//.
+            rewrite /new_dom. apply elem_of_difference; split.
+            ** apply elem_of_dom_2 in Hin. rewrite ls_same_doms in Hin. set_solver.
+            ** assert (ρ ∉ dom fs); last set_solver. rewrite dom_fmap_L in Hxdom.
+               intros contra%Hxdom. congruence.
+      - intros ζ0 Hnotin. apply lookup_insert_None; split.
+        + apply Hlocssmall.
+          destruct (trace_last extr).
+          have ? := locales_of_list_step_incl _ _ _ _ _ Hstep. simpl.
+          clear Hfueldom Hsamedoms. set_solver.
+        + intros <-.
+          destruct (trace_last extr).
+          have ? := locales_of_list_step_incl _ _ _ _ _ Hstep. simpl.
+          clear Hfueldom Hsamedoms. inversion Hstep. simplify_eq.
+          assert (locale_of t1 e1 ∈ locales_of_list (t1 ++ e1 :: t2)); last set_solver.
+          apply locales_of_list_from_locale_from.
+          rewrite from_locale_from_Some // prefixes_from_spec. eexists _,_. by list_simplifier.
+      - rewrite Hnewdom /new_dom. apply elem_of_equiv_empty_L. intros ρ [Hin1 Hin2]%elem_of_intersection.
+        assert (ρ ∈ dom (ls_fuel (trace_last auxtr))) by set_solver. set_solver. }
+    iPureIntro.
+    do 2 split; first done. split; [split; [|split; [|split; [|split]]]|] =>//.
+    - eexists. apply Hxdom. by rewrite dom_fmap.
+    - unfold fuel_decr. simpl.
+      intros ρ' Hin Hin' Hmustdec.
+      rewrite Hnewdom in Hin'.
+
       inversion Hmustdec; simplify_eq.
-      have Hin: ρ' ∈ dom (S <$> fs) by set_solver.
-      rewrite map_lookup_imap Hfuel // lookup_fmap.
-      destruct (S <$> fs !! ρ') as [f|] eqn:Heq; simpl.
-      + rewrite decide_True //; last by set_solver.
-        destruct (fs!!ρ') as [f'|]=> //=.
-        simpl in Heq. injection Heq=>Heq'. rewrite -Heq'.
-        rewrite lookup_gset_to_gmap option_guard_True /=; last by set_solver. lia.
-      + have: ρ' ∉ dom (S <$> fs).
-        { apply not_elem_of_dom. rewrite lookup_fmap //. }
-        set_solver. }
-    iPureIntro. split=>//. intros ρ' Hin _.
-    rewrite map_lookup_imap. rewrite -ls_fuel_dom in Hin.
-    apply elem_of_dom in Hin as [f Hf]. rewrite Hf /=.
-    destruct (decide (ρ' ∈ dom fs)).
-    + rewrite lookup_gset_to_gmap option_guard_True /=; last by set_solver.
-      rewrite -Hf Hfuel; last set_solver. rewrite lookup_fmap.
-      destruct (fs!!ρ') as [f'|] eqn:Heq'; first (simpl; lia).
-      rewrite Hfuel in Hf; last set_solver. rewrite lookup_fmap Heq' // in Hf.
-    + assert (ρ' ∈ dom (ls_fuel (trace_last auxtr))).
-      { apply elem_of_dom. eexists _; done. }
-      rewrite lookup_gset_to_gmap option_guard_True /=; [lia | set_solver].
+      + have Hinfs: ρ' ∈ dom (S <$> fs) by set_solver.
+        rewrite map_lookup_imap Hfuel // lookup_fmap. rewrite dom_fmap in Hinfs.
+        rewrite lookup_gset_to_gmap option_guard_True //=.
+
+        pose proof Hinfs as Hinfs'. apply elem_of_dom in Hinfs' as [f Heqf].
+        assert (filter (λ '(k, _), k ∈ dom fs ∖ rem) fs !! ρ' = Some f) as Heqfilter.
+        { rewrite map_filter_lookup Heqf /= option_guard_True //. set_solver. }
+        rewrite decide_True // ?Heqfilter ?lookup_fmap ?Heqf /=; last by eapply elem_of_dom_2. lia.
+      + rewrite /= /new_mapping map_filter_lookup in Hneqtid.
+        pose proof Hin as Hin2. rewrite -ls_same_doms in Hin2. apply elem_of_dom in Hin2 as [f Hf].
+        rewrite Hf /= option_guard_True // in Hneqtid.
+    - intros ρ' Hin _. simpl. destruct (decide (ρ' ∈ rem)) as [Hin'|Hnin'].
+      + right; split; last set_solver. rewrite /fuel_apply map_imap_dom_eq ?dom_gset_to_gmap; first set_solver.
+        intros ρ0 _ Hin0. destruct (decide (ρ0 ∈ dom (filter (λ '(k, _), k ∈ dom fs ∖ rem) fs))) as [?|Hnin];
+          first by apply elem_of_dom.
+        apply elem_of_difference in Hin0 as [Hin1 ?].
+        apply elem_of_union in Hin1 as [?|Hin2]; first by apply elem_of_dom.
+        exfalso. apply Hnin. apply elem_of_dom in Hin2 as [f ?].
+        eapply elem_of_dom_2. rewrite map_filter_lookup_Some. split =>//.
+        apply elem_of_difference; split =>//. by eapply elem_of_dom_2.
+      + left. rewrite map_lookup_imap lookup_gset_to_gmap option_guard_True //=; last set_solver.
+        apply elem_of_dom in Hin as [f Hf].
+        destruct (decide (ρ' ∈ dom (filter (λ '(k, _), k ∈ dom fs ∖ rem) fs))) as [Hin|?];
+          last by rewrite !Hf //=.
+        apply elem_of_dom in Hin as [f' Hf']. rewrite Hf'.
+        apply map_filter_lookup_Some in Hf' as [Hfs Hf'].
+        rewrite Hfuel ?lookup_fmap ?Hfs /=; [lia |]. rewrite dom_fmap; set_solver.
+    - rewrite Hnewdom. assert (dom fs ⊆ dom $ ls_fuel (trace_last auxtr)); last set_solver.
+        intros ρ Hin. apply elem_of_dom. rewrite Hfuel ?dom_fmap // -elem_of_dom dom_fmap //.
+    - unfold tids_smaller; simpl. intros ρ ζ0 Hin.
+      destruct (trace_last extr); destruct (trace_last extr).
+      eapply from_locale_step =>//.
+      rewrite /tids_smaller /= in Hζs. eapply Hζs.
+      rewrite /new_mapping map_filter_lookup_Some in Hin.
+      by destruct Hin.
   Qed.
 
   Lemma update_fork_split R1 R2 tp1 tp2 fs (extr : execution_trace Λ)
@@ -822,11 +918,11 @@ Section model_state_lemmas.
     iDestruct (has_fuel_fuel with "Hf Hmod") as %Hfuels.
 
     iDestruct (model_state_interp_tids_smaller with "Hmod") as %Hts.
-    iDestruct "Hmod" as (M) "(Haf&Ham&%Hminv&%Hsmall&Hamod)".
+    iDestruct "Hmod" as (M FR) "(Haf&Ham&HFR&%Hminv&%Hsmall&Hamod&%HFR)".
 
     pose Hlocincl := locales_of_list_step_incl _ _ _ _ _ Hstep.
 
-    iMod (update_has_fuels_no_step ζ (S <$> fs) fs with "Hf Haf Ham") as "(Haf&Hf&Ham)".
+    iMod (update_has_fuels_no_step_no_change ζ (S <$> fs) fs with "Hf Haf Ham") as "(Haf&Hf&Ham)".
     { intros contra. apply fmap_empty_inv in contra. set_solver. }
     { rewrite dom_fmap_L //. }
 
@@ -846,29 +942,33 @@ Section model_state_lemmas.
       apply prefixes_from_spec.
       exists t0, []. split =>//. by list_simplifier. }
 
-    iMod (update_mapping_new_locale ζ _ _ R1 R2 with "Ham Hf") as "(Ham&HR1&HR2)"; eauto.
+    iMod (update_mapping_new_locale ζ (locale_of tp1 efork) _ R1 R2 with "Ham Hf") as "(Ham&HR1&HR2)"; eauto.
 
     pose δ1 := trace_last auxtr.
-    assert (Hfueldom: dom (map_imap
-                             (λ ρ o,
-                              if decide (ρ ∈ R1 ∪ R2) then Some (o - 1)%nat else Some o)
-                             (ls_fuel δ1)) = live_roles Mdl δ1).
-    { rewrite map_imap_dom_eq; first rewrite ls_fuel_dom //.
-      intros ρ f Hin. destruct (decide (ρ ∈ R1 ∪ R2)); eauto. }
-    assert (Hmappingdom: dom (map_imap
+    assert (Hsamedoms: dom (map_imap
                                 (λ ρ o,
                                  if decide (ρ ∈ R2) then Some $ locale_of tp1 efork else Some o)
-                                (ls_mapping δ1)) = live_roles Mdl δ1).
-    { rewrite map_imap_dom_eq; first rewrite ls_mapping_dom //.
-      intros ρ f Hin. destruct (decide (ρ ∈ R2)); eauto. }
+                                (ls_mapping δ1)) =
+                         dom (map_imap
+                             (λ ρ o,
+                              if decide (ρ ∈ R1 ∪ R2) then Some (o - 1)%nat else Some o)
+                             (ls_fuel δ1))
+           ).
+    { rewrite !map_imap_dom_eq; first by rewrite ls_same_doms.
+      - by intros ρ??; destruct (decide (ρ ∈ R1 ∪ R2)).
+      - by intros ρ??; destruct (decide (ρ ∈ R2)). }
+    assert (Hfueldom: live_roles _ δ1 ⊆ dom (map_imap
+                             (λ ρ o,
+                              if decide (ρ ∈ R1 ∪ R2) then Some (o - 1)%nat else Some o)
+                             (ls_fuel δ1))).
+    { rewrite map_imap_dom_eq; first by apply ls_fuel_dom.
+      - by intros ρ??; destruct (decide (ρ ∈ R1 ∪ R2)). }
     iExists {|
       ls_under := δ1.(ls_under);
-      ls_fuel :=
-        map_imap (λ ρ o, if (decide (ρ ∈ R1 ∪ R2)) then Some (o-1)%nat else Some o) (ls_fuel δ1);
+      ls_fuel := _;
       ls_fuel_dom := Hfueldom;
-      ls_mapping :=
-        map_imap (λ ρ o, if (decide (ρ ∈ R2)) then Some $ locale_of tp1 efork else Some o) (ls_mapping δ1);
-      ls_mapping_dom := Hmappingdom;
+      ls_mapping := _;
+      ls_same_doms := Hsamedoms;
     |}.
     iModIntro.
     assert (Hdomincl: dom fs ⊆ dom (ls_fuel δ1)).
@@ -884,8 +984,8 @@ Section model_state_lemmas.
     { unfold has_fuels. rewrite dom_domain_restrict; [|set_solver]. iFrame.
       iApply (big_sepS_impl with "Hf1"). iIntros "!#" (x Hin) "(%f&%&?)".
       iExists _; iFrame. iPureIntro. rewrite map_filter_lookup_Some //. }
-    iSplitL "Ham Haf Hamod".
-    { iExists _; simpl. iFrame "Ham Hamod".
+    iSplitL "Ham Haf Hamod HFR".
+    { iExists _, FR; simpl. iFrame "Ham Hamod HFR".
       iSplit.
       - iApply (auth_fuel_is_proper with "Haf"). unfold fuel_apply.
         rewrite -leibniz_equiv_iff. intros ρ. rewrite !map_lookup_imap.
@@ -907,10 +1007,10 @@ Section model_state_lemmas.
         + rewrite option_guard_False //=.
           rewrite -> not_elem_of_union in Hin. destruct Hin as [Hin ?].
           rewrite -> not_elem_of_dom in Hin. rewrite Hin //.
-      - iPureIntro. split; last first.
+      - iPureIntro. split; first last; [split|].
         { intros ζ' Hζ'. rewrite lookup_insert_ne; last first.
           { pose proof (locales_of_list_step_incl _ _ _ _ _ Hstep).
-            clear Hfueldom Hmappingdom.
+            clear Hfueldom Hsamedoms.
             assert (ζ' ∉ locales_of_list tp1); first by set_solver.
             intros contra. simplify_eq.
             destruct Htlen as [tp1' [-> Hlen]].
@@ -930,7 +1030,7 @@ Section model_state_lemmas.
           rewrite lookup_insert_ne; last first.
           { intros <-. rewrite Hsmall in Hmapping; [congruence | set_solver]. }
           apply Hsmall; set_solver.  }
-
+        { rewrite map_imap_dom_eq // => ρ f Hin. by destruct (decide (ρ ∈ R1 ∪ R2)). }
         intros ρ ζ'. rewrite map_lookup_imap.
         destruct (decide (ρ ∈ dom (ls_mapping δ1))) as [Hin|Hin].
         + apply elem_of_dom in Hin as [ζ'' Hρ]. rewrite Hρ. simpl.
@@ -971,7 +1071,7 @@ Section model_state_lemmas.
                { eapply Hminv. eexists _. split; eauto. }
                congruence.
         + apply not_elem_of_dom in Hin. rewrite Hin /=. split; first done.
-          intros (?&Hin'&?). rewrite ls_fuel_dom -ls_mapping_dom in Hdomincl.
+          intros (?&Hin'&?). rewrite -ls_same_doms in Hdomincl.
           apply not_elem_of_dom in Hin.
           destruct (decide (ζ' = locale_of tp1 efork)).
           { simplify_eq. rewrite lookup_insert in Hin'. simplify_eq. set_solver. }
@@ -983,14 +1083,39 @@ Section model_state_lemmas.
           { eapply Hminv. eauto. }
           apply not_elem_of_dom in Hin. congruence. }
     iSplit; first done.
-    iSplit; [iSplit|].
+    iSplit; last first.
+    { iPureIntro. intros ρ ζ'. simpl. rewrite map_lookup_imap.
+      destruct (ls_mapping δ1 !!ρ) eqn:Heq; last done. simpl.
+      destruct (decide (ρ ∈ R2)); first  (intros ?; simplify_eq).
+      - destruct Htlen as [tp1' [-> Hlen]].
+        inversion Hstep as [? ? e1 ? e2 ? efs t1 t2 Hf1 YY Hprimstep |]. simplify_eq.
+        assert (efs = [efork]) as ->.
+        { symmetry. assert (length tp1' = length (t1 ++ e2 :: t2)).
+          rewrite app_length //=; rewrite app_length //= in Hlen.
+          clear Hlen. eapply app_inj_1 =>//. by list_simplifier. }
+        assert (is_Some (from_locale (t1 ++ e1 :: t2 ++ [efork]) (locale_of (t1 ++ e1 :: t2) efork))).
+        + unfold from_locale. erewrite from_locale_from_Some; eauto.
+          apply prefixes_from_spec. list_simplifier. eexists _, []. split=>//.
+          by list_simplifier.
+        + eapply from_locale_from_equiv =>//; [constructor |]. rewrite H1.
+          replace (t1 ++ e1 :: t2 ++ [efork]) with ((t1 ++ e1 :: t2) ++ [efork]);
+            last by list_simplifier.
+          replace (t1 ++ e2 :: t2 ++ [efork]) with ((t1 ++ e2 :: t2) ++ [efork]);
+            last by list_simplifier.
+          assert (locales_equiv (t1 ++ e1 :: t2) (t1 ++ e2 :: t2)).
+          { apply locales_equiv_middle. eapply locale_step_preserve =>//. }
+          apply locales_equiv_from_app =>//. by eapply locales_from_equiv_refl.
+      - intros ?; simplify_eq.
+        assert (is_Some (from_locale tp1 ζ')) by eauto.
+        eapply from_locale_step =>//. }
+    iSplit.
     { iPureIntro. destruct (map_choose _ Hnemp) as [ρ[??]]. exists ρ.
       apply Hminv. eexists _. split; eauto. apply elem_of_dom. eauto. }
     iSplit.
-    { iPureIntro. intros ρ Hlive Hmd. simpl. inversion Hmd; simplify_eq.
+    { iPureIntro. intros ρ Hlive Hlive' Hmd. simpl. inversion Hmd; simplify_eq.
       - rewrite map_lookup_imap.
         assert (Hin: ρ ∈ dom (ls_fuel δ1)).
-        { rewrite ls_fuel_dom -ls_mapping_dom elem_of_dom. eauto. }
+        { rewrite -ls_same_doms elem_of_dom. eauto. }
         apply elem_of_dom in Hin. destruct Hin as [f' Hin'].
         rewrite Hin' /=.
         destruct (decide (ρ ∈ R1 ∪ R2)) as [Hin''|Hin''].
@@ -1008,257 +1133,309 @@ Section model_state_lemmas.
         rewrite Hfuels; last set_solver. rewrite lookup_fmap.
         assert (Hindom: ρ ∈ dom fs); first by set_solver.
         apply elem_of_dom in Hindom as [f Hindom]. rewrite Hindom /= decide_True /=; [lia|set_solver]. }
-    iSplit; last done.
-    { iPureIntro. intros ρ' Hρ' _. simpl.
-      rewrite map_lookup_imap. rewrite <-ls_fuel_dom, elem_of_dom in Hρ'.
+    iSplit.
+    { iPureIntro. intros ρ' Hρ' _. simpl. left.
+      rewrite map_lookup_imap. rewrite elem_of_dom in Hρ'.
       destruct Hρ' as [f Hf]. rewrite Hf /=. destruct (decide ((ρ' ∈ R1 ∪ R2))); simpl; lia. }
-    iPureIntro. intros ρ ζ'. simpl. rewrite map_lookup_imap.
-    destruct (ls_mapping δ1 !!ρ) eqn:Heq; last done. simpl.
-    destruct (decide (ρ ∈ R2)); first  (intros ?; simplify_eq).
-    - destruct Htlen as [tp1' [-> Hlen]].
-      inversion Hstep as [? ? e1 ? e2 ? efs t1 t2 Hf1 YY Hprimstep |]. simplify_eq.
-      assert (efs = [efork]) as ->.
-      { symmetry. assert (length tp1' = length (t1 ++ e2 :: t2)).
-        rewrite app_length //=; rewrite app_length //= in Hlen.
-        clear Hlen. eapply app_inj_1 =>//. by list_simplifier. }
-      assert (is_Some (from_locale (t1 ++ e1 :: t2 ++ [efork]) (locale_of (t1 ++ e1 :: t2) efork))).
-      + unfold from_locale. erewrite from_locale_from_Some; eauto.
-        apply prefixes_from_spec. list_simplifier. eexists _, []. split=>//.
-        by list_simplifier.
-      + eapply from_locale_from_equiv =>//; [constructor |]. rewrite H1.
-        replace (t1 ++ e1 :: t2 ++ [efork]) with ((t1 ++ e1 :: t2) ++ [efork]);
-          last by list_simplifier.
-        replace (t1 ++ e2 :: t2 ++ [efork]) with ((t1 ++ e2 :: t2) ++ [efork]);
-          last by list_simplifier.
-        assert (locales_equiv (t1 ++ e1 :: t2) (t1 ++ e2 :: t2)).
-        { apply locales_equiv_middle. eapply locale_step_preserve =>//. }
-        apply locales_equiv_from_app =>//. by eapply locales_from_equiv_refl.
-    - intros ?; simplify_eq.
-      assert (is_Some (from_locale tp1 ζ')) by eauto.
-      eapply from_locale_step =>//.
+    iSplit; [simpl| done]. rewrite map_imap_dom_eq //.
+    by intros ρ??; destruct (decide (ρ ∈ R1 ∪ R2)).
   Qed.
 
   Definition valid_new_fuelmap (fs1 fs2: gmap (fmrole Mdl) nat) (s1 s2: Mdl) (ρ: fmrole Mdl) :=
     (ρ ∈ live_roles _ s2 -> oleq (fs2 !! ρ) (Some (fuel_limit s2))) ∧
+    (ρ ∉ live_roles _ s2 -> ρ ∈ dom fs1 ∩ dom fs2 -> oless (fs2 !! ρ) (fs1 !! ρ)) ∧
     ρ ∈ dom fs1 ∧
-    (forall ρ', ρ' ∈ dom fs2 ∖ live_roles _ s1 -> oleq (fs2 !! ρ') (Some $ fuel_limit s2)) ∧
+    (forall ρ', ρ' ∈ dom fs2 ∖ dom fs1 -> oleq (fs2 !! ρ') (Some $ fuel_limit s2)) ∧
     (forall ρ', ρ ≠ ρ' -> ρ' ∈ dom fs1 ∩ dom fs2 -> oless (fs2 !! ρ') (fs1 !! ρ')) ∧
-    dom fs2 = (dom fs1 ∩ live_roles _ s2) ∪ (live_roles _ s2 ∖ live_roles _ s1).
+    (dom fs1 ∖ {[ ρ ]}) ∪ (live_roles _ s2 ∖ live_roles _ s1) ⊆ dom fs2 ∧
+    dom fs2 ⊆
+      (* new roles *) (live_roles _ s2 ∖ live_roles _ s1) ∪
+      (* surviving roles *) (live_roles _ s2 ∩ live_roles _ s1 ∩ dom fs1) ∪
+      (* already dead *) (dom fs1 ∖ live_roles _ s1) ∪
+      (* new deads *) ((live_roles _ s1 ∖ live_roles _ s2) ∩ dom fs1).
+
+  Ltac by_contradiction :=
+    match goal with
+    | |- ?goal => destruct_decide (decide (goal)); first done; exfalso
+    end.
 
   Lemma update_step_still_alive
         (extr : execution_trace Λ)
         (auxtr: auxiliary_trace (fair_model Mdl))
-        tp1 tp2 σ1 σ2 s1 s2 fs1 fs2 ρ (δ1 : fair_model Mdl) ζ:
+        tp1 tp2 σ1 σ2 s1 s2 fs1 fs2 ρ (δ1 : fair_model Mdl) ζ fr1:
+    (live_roles _ s2 ∖ live_roles _ s1) ⊆ fr1 ->
     trace_last extr = (tp1, σ1) →
     trace_last auxtr = δ1 ->
     locale_step (tp1, σ1) (Some ζ) (tp2, σ2) ->
     fmtrans _ s1 (Some ρ) s2 -> valid_new_fuelmap fs1 fs2 δ1 s2 ρ ->
-    has_fuels ζ fs1 -∗ frag_model_is s1 -∗ model_state_interp tp1 δ1
+    has_fuels ζ fs1 -∗ frag_model_is s1 -∗ model_state_interp tp1 δ1 -∗
+    frag_free_roles_are fr1
     ==∗ ∃ (δ2: fair_model Mdl) ℓ,
         ⌜labels_match (Some ζ) ℓ
         ∧ valid_state_evolution_fairness (extr :tr[Some ζ]: (tp2, σ2)) (auxtr :tr[ℓ]: δ2)⌝
-        ∗ has_fuels ζ fs2 ∗ frag_model_is s2 ∗ model_state_interp tp2 δ2.
+        ∗ has_fuels ζ fs2 ∗ frag_model_is s2 ∗ model_state_interp tp2 δ2 ∗
+        frag_free_roles_are (fr1 ∖ (live_roles _ s2 ∖ live_roles _ s1)).
   Proof.
-    iIntros (Htrlast Hauxtrlast Hstep Htrans Hfuelsval) "Hfuel Hmod Hsi".
+    iIntros (Hfr_new Htrlast Hauxtrlast Hstep Htrans Hfuelsval) "Hfuel Hmod Hsi Hfr1".
 
     assert (Hfsne: fs1 ≠ ∅).
-    { destruct Hfuelsval as (_&?&_). intros ->. set_solver. }
+    { destruct Hfuelsval as (_&_&?&_). intros ->. set_solver. }
 
     iDestruct (has_fuel_in with "Hfuel Hsi") as "%Hxdom"; eauto.
     iDestruct (has_fuel_fuel with "Hfuel Hsi") as %Hfuel; eauto.
     iDestruct (model_state_interp_tids_smaller with "Hsi") as %Hless.
 
-    iDestruct "Hsi" as "(%M&Hafuel&Hamapping&%Hinv&%Hsmall&Hamod)".
+    iDestruct "Hsi" as "(%M&%FR&Hafuel&Hamapping&HFR&%Hinv&%Hsmall&Hamod&%HFR)".
     iDestruct (model_agree with "Hamod Hmod") as "%Heq".
 
-    assert (Hfueldom: dom (update_fuel_resource δ1 fs2 s2) = live_roles Mdl s2).
+    iDestruct (free_roles_inclusion with "HFR Hfr1") as %HfrFR.
+
+    assert (Hsamedoms:
+             dom (map_imap
+                    (λ ρ' _, if decide (ρ' ∈ dom $ ls_fuel δ1) then ls_mapping δ1 !! ρ' else Some ζ)
+                    (gset_to_gmap 333 ((dom (ls_fuel δ1) ∪ dom fs2) ∖ (dom fs1 ∖ dom fs2)))) =
+               dom (update_fuel_resource δ1 fs1 fs2 s2)).
     { unfold update_fuel_resource, fuel_apply. rewrite -leibniz_equiv_iff.
       intros ρ'; split.
-      - intros [f Hin]%elem_of_dom. rewrite map_lookup_imap in Hin.
-        destruct (decide (ρ' ∈ live_roles _ s2)); first done.
-        rewrite lookup_gset_to_gmap option_guard_False // in Hin.
       - intros Hin. destruct (decide (ρ' ∈ dom fs2)) as [[f Hin1]%elem_of_dom|Hin1].
         + apply elem_of_dom. eexists f. rewrite map_lookup_imap lookup_gset_to_gmap option_guard_True //=.
           rewrite decide_True //. apply elem_of_dom. rewrite Hin1; eauto.
-        + apply elem_of_dom. rewrite map_lookup_imap lookup_gset_to_gmap option_guard_True //=.
-          rewrite decide_False //. apply elem_of_dom. rewrite ls_fuel_dom.
-          destruct Hfuelsval as (?&?&?&?&Hdomeq). rewrite Hdomeq in Hin1. set_solver. }
+          rewrite map_imap_dom_eq dom_gset_to_gmap in Hin; first set_solver.
+          intros ρ0??. destruct (decide (ρ0 ∈ dom $ ls_fuel δ1)); [|done].
+          apply elem_of_dom. rewrite ls_same_doms. SS.
+        + rewrite map_imap_dom_eq dom_gset_to_gmap; last first.
+          { intros ρ0 ? Hin0. destruct (decide (ρ0 ∈ dom fs2)) as [|Hnotin]; apply elem_of_dom; first done.
+            unfold valid_new_fuelmap in Hfuelsval.
+            destruct Hfuelsval as (_&_&_&_& Hdomfs2). set_solver. }
 
-    assert (Hmappingdom: dom (map_imap
-                                  (λ ρ' _, if decide (ρ' ∈ live_roles Mdl δ1) then ls_mapping δ1 !! ρ' else Some ζ)
-                                  (gset_to_gmap 333 (live_roles Mdl s2))) = live_roles Mdl s2).
-    { rewrite -leibniz_equiv_iff. intros ρ'; split.
+          rewrite map_imap_dom_eq dom_gset_to_gmap in Hin; first set_solver.
+          intros ρ0??. destruct (decide (ρ0 ∈ dom $ ls_fuel δ1)); [|done].
+          apply elem_of_dom. rewrite ls_same_doms. SS.
       - intros [f Hin]%elem_of_dom. rewrite map_lookup_imap in Hin.
-        destruct (decide (ρ' ∈ live_roles _ s2)); first done.
-        rewrite lookup_gset_to_gmap option_guard_False // in Hin.
-      - intros Hin. destruct (decide (ρ' ∈ live_roles _ δ1)) as [Hin1|Hin1].
-        + apply elem_of_dom. rewrite map_lookup_imap lookup_gset_to_gmap option_guard_True //=.
-          rewrite decide_True //. apply elem_of_dom. rewrite ls_mapping_dom //.
-        + apply elem_of_dom. rewrite map_lookup_imap lookup_gset_to_gmap option_guard_True //=.
-          rewrite decide_False //. }
+        rewrite map_imap_dom_eq dom_gset_to_gmap.
+        + by_contradiction. rewrite lookup_gset_to_gmap option_guard_False // in Hin.
+        + intros ρ0??. destruct (decide (ρ0 ∈ dom $ ls_fuel δ1)); [|done].
+          apply elem_of_dom. rewrite ls_same_doms. SS. }
+
+    assert (Hnewdom: dom (update_fuel_resource δ1 fs1 fs2 s2) =
+                       (dom (ls_fuel δ1) ∪ dom fs2) ∖ (dom fs1 ∖ dom fs2)).
+    { unfold update_fuel_resource, fuel_apply. rewrite map_imap_dom_eq ?dom_gset_to_gmap //.
+      intros ρ' _ Hin. destruct (decide (ρ' ∈ dom fs2)); apply elem_of_dom =>//. set_solver. }
+
+    assert (Hfueldom: live_roles _ s2 ⊆ dom $ update_fuel_resource δ1 fs1 fs2 s2).
+    { rewrite -Hsamedoms map_imap_dom_eq dom_gset_to_gmap //.
+      { epose proof ls_fuel_dom. intros ρ' Hin.
+        destruct Hfuelsval as (?&?&?&?&?&?).
+        destruct (decide (ρ' ∈ live_roles _ δ1)).
+        - apply elem_of_difference; split; [set_solver|].
+          intros [? Habs]%elem_of_difference.
+          destruct (decide (ρ' = ρ)).
+          + simplify_eq. apply not_elem_of_dom in Habs.
+            rewrite -> Habs in *. simpl in *. eauto.
+          + apply Habs. assert (ρ' ∈ dom fs1 ∖ {[ρ]}); set_solver.
+        - apply elem_of_difference; split; [apply elem_of_union; right; set_solver|set_solver]. }
+      intros ρ0??. destruct (decide (ρ0 ∈ dom $ ls_fuel δ1)); [|done].
+      apply elem_of_dom. rewrite ls_same_doms. SS. }
 
     iExists {|
       ls_under := s2;
-      ls_fuel := update_fuel_resource δ1 fs2 s2;
+      ls_fuel :=  _;
       ls_fuel_dom := Hfueldom;
-      ls_mapping := map_imap
-                      (λ ρ' fold, if decide (ρ' ∈ live_roles _ δ1)
-                                  then δ1.(ls_mapping) !! ρ'
-                                  else Some ζ)
-                      (gset_to_gmap 333 (live_roles _ s2));
-      ls_mapping_dom := Hmappingdom;
+      ls_mapping := _;
+      ls_same_doms := Hsamedoms;
     |}, (Take_step ρ ζ).
     Unshelve.
     iMod (update_has_fuels _ fs1 fs2 with "Hfuel Hafuel Hamapping") as "(Hafuel & Hfuel & Hmapping)".
     { set_solver. }
     { unfold valid_new_fuelmap in Hfuelsval.
-      destruct Hfuelsval as (_&_&?&?&->). rewrite !Heq.
-      rewrite ls_fuel_dom. set_solver. }
+      destruct Hfuelsval as (_&_&?&?& Hfs2_inf&Hfs2_sup).
+
+      apply elem_of_equiv_empty_L => ρ0 Hin.
+      apply elem_of_intersection in Hin as [Hin1 Hin2].
+      apply elem_of_difference in Hin1 as [Hin11 Hin12].
+
+      assert (ρ0 ∈ live_roles _ s2 ∖ live_roles _ s1) by set_solver.
+      assert (ρ0 ∈ fr1) by set_solver.
+      assert (ρ0 ∈ FR) by set_solver.
+      assert (ρ0 ∉ dom (ls_fuel δ1)) by set_solver.
+      done. }
     iMod (update_model s2 with "Hamod Hmod") as "[Hamod Hmod]".
+    iMod (update_free_roles (live_roles Mdl s2 ∖ live_roles Mdl s1)
+           with "HFR Hfr1") as "[HFR Hfr2]"; [set_solver|].
     iModIntro. iSplit.
     { iSplit; first done. iPureIntro.
-      destruct Hfuelsval as (Hlim&Hinfs1m&Hnewlim&Hdec&Hdomeq).
+      destruct Hfuelsval as (Hlim&Hzombie&Hinfs1m&Hnewlim&Hdec&Hinf&Hsup).
       constructor =>//; split.
       - constructor; simpl; first by rewrite Hauxtrlast Heq //.
         split; first by rewrite Hauxtrlast; apply Hxdom; set_solver.
         split.
-        { intros ?? Hmd. inversion Hmd; clear Hmd; simplify_eq.
+        { intros ??? Hmd. inversion Hmd; clear Hmd; simplify_eq.
           + symmetry in Hsametid. rewrite -> Hxdom in Hsametid. simpl.
             unfold update_fuel_resource, fuel_apply.
             rewrite map_lookup_imap lookup_gset_to_gmap.
-            destruct (decide (ρ' ∈ live_roles Mdl s2)) as [Hin|Hin].
+            destruct (decide (ρ' ∈ live_roles Mdl s2 ∪ dom fs2)) as [Hin|Hin].
             * rewrite option_guard_True //=.
               { destruct (decide (ρ' ∈ dom fs2)) as [Hin2|Hin2].
                 ** rewrite Hfuel; last set_solver. apply Hdec; [congruence|set_solver].
                 ** exfalso. set_solver. }
+              apply elem_of_difference; split; [set_solver|].
+              apply not_elem_of_difference; right.
+              apply elem_of_union in Hin as [|]; [|done].
+              destruct (decide (ρ' = ρ)); simplify_eq.
+              apply Hinf; set_solver.
             * rewrite option_guard_False //=.
-              eapply Hin, fm_live_preserved; [done| | congruence].
-              rewrite <-Hxdom in Hsametid. rewrite -ls_mapping_dom elem_of_dom. by eauto.
+              ** assert (ρ' ∈ dom fs2); set_solver.
+              ** apply not_elem_of_difference; right; set_solver.
           + simpl in *. unfold update_fuel_resource, fuel_apply.
             rewrite map_lookup_imap lookup_gset_to_gmap.
-            destruct (decide (ρ' ∈ live_roles Mdl s2)) as [Hin|Hin].
-            * rewrite option_guard_True //=.
-              { destruct (decide (ρ' ∈ dom fs2)) as [Hin2|Hin2].
-                ** rewrite Hfuel; last set_solver.
-                   rewrite Hdomeq in Hin2. exfalso.
-                   assert (Hin3: ρ' ∈ dom fs1).
-                   { set_solver. }
-                   rewrite map_lookup_imap in Hneqtid.
-                   rewrite <-Hxdom in Hin3.
-                   rewrite Hin3 /= in Hneqtid.
-                   rewrite lookup_gset_to_gmap option_guard_True //= in Hneqtid.
-                   rewrite decide_True // in Hneqtid.
-                ** rewrite map_lookup_imap in Hneqtid.
-                   assert (is_Some (ls_mapping (trace_last auxtr) !! ρ')) as [ζ' Hζ'].
-                   { apply elem_of_dom. rewrite ls_mapping_dom //. }
-                   rewrite lookup_gset_to_gmap option_guard_True //= in Hneqtid.
-                   rewrite Hζ' /= decide_True // in Hneqtid. }
-            * rewrite option_guard_False //=.
-              rewrite map_lookup_imap in Hissome.
-              assert (is_Some (ls_mapping (trace_last auxtr) !! ρ')) as [ζ' Hζ'].
-              { apply elem_of_dom. rewrite ls_mapping_dom //. }
-              rewrite lookup_gset_to_gmap option_guard_False //= in Hissome.
-                by inversion Hissome. }
+
+            destruct (decide (ρ' ∈ (dom (ls_fuel (trace_last auxtr)) ∪ dom fs2) ∖ (dom fs1 ∖ dom fs2))) as [Hin|Hin].
+            * rewrite map_lookup_imap lookup_gset_to_gmap option_guard_True //= decide_True //= in Hneqtid.
+            * apply not_elem_of_difference in Hin as [?|Hin]; [set_solver|].
+              apply elem_of_difference in Hin as [??].
+              rewrite map_lookup_imap lookup_gset_to_gmap /= option_guard_False /= in Hissome;
+                [inversion Hissome; congruence|set_solver].
+          + simpl in *. rewrite Hfuel; last set_solver. unfold update_fuel_resource, fuel_apply.
+            rewrite Hnewdom in Hnotdead. rewrite map_lookup_imap lookup_gset_to_gmap option_guard_True //=.
+            assert (ρ' ∈ dom fs2) by set_solver.
+            rewrite decide_True; [apply Hzombie =>//; set_solver | done]. }
         split.
         + intros ? Hin ?. simplify_eq; simpl.
           unfold update_fuel_resource, fuel_apply.
           rewrite map_lookup_imap lookup_gset_to_gmap.
-          destruct (decide (ρ' ∈ live_roles _ s2)) as [Hlive|Hlive].
+          destruct (decide (ρ' ∈ (dom (ls_fuel (trace_last auxtr)) ∪ dom fs2) ∖ (dom fs1 ∖ dom fs2))) as [Hlive|Hlive].
           * rewrite option_guard_True //=.
+            apply elem_of_difference in Hlive as [Hin1 Hnin].
+            apply not_elem_of_difference in Hnin.
+
             destruct (decide (ρ' ∈ dom fs2)) as [Hin2|Hin2].
-            ** rewrite Hfuel; last set_solver. apply oleq_oless, Hdec; [congruence|set_solver].
-            ** rewrite <-ls_fuel_dom, elem_of_dom in Hin. destruct Hin as [? ->]. simpl;lia.
-          * rewrite option_guard_False //=.
-            eapply Hlive, fm_live_preserved =>//. congruence.
+            ** destruct (decide (ρ' ∈ live_roles _ (trace_last auxtr)));left.
+               *** destruct (decide (ρ' ∈ dom fs1)).
+                   { rewrite Hfuel //. apply oleq_oless, Hdec; [congruence|set_solver]. }
+                   { exfalso. set_solver. }
+               *** assert (ρ' ∉ live_roles _ s2).
+                   { by_contradiction. assert (ρ' ∈ fr1); [eapply elem_of_subseteq; eauto; set_solver|].
+                     assert (ρ' ∈ FR); [eapply elem_of_subseteq; eauto; set_solver|set_solver]. }
+                   assert (ρ' ∈ dom fs1). set_solver.
+                   rewrite Hfuel //. apply oleq_oless, Hdec; [congruence|set_solver].
+            ** left. rewrite elem_of_dom in Hin. destruct Hin as [? ->]. simpl;lia.
+          * right; split.
+            ** eapply not_elem_of_weaken; [|by apply map_imap_dom_inclusion; rewrite dom_gset_to_gmap].
+               rewrite dom_gset_to_gmap //.
+            ** apply not_elem_of_difference in Hlive as [?|Hlive]; [set_solver|].
+               apply elem_of_difference in Hlive as [? Habs].
+               exfalso. apply Habs. set_solver.
         + split.
           { intros Hlive. unfold update_fuel_resource, fuel_apply.
-            rewrite map_lookup_imap lookup_gset_to_gmap option_guard_True //=.
-            rewrite decide_True; [by apply Hlim | set_solver]. }
-          intros ??. unfold update_fuel_resource, fuel_apply.
-          rewrite map_lookup_imap lookup_gset_to_gmap option_guard_True //=; last set_solver.
-          rewrite decide_True; first apply Hnewlim; set_solver.
+          destruct (decide (ρ ∈ (dom (ls_fuel (trace_last auxtr)) ∪ dom fs2) ∖ (dom fs1 ∖ dom fs2))) as [Hin|Hnin].
+          - rewrite map_lookup_imap lookup_gset_to_gmap option_guard_True //=; last set_solver.
+            rewrite decide_True; [by apply Hlim |set_solver].
+          - exfalso; apply not_elem_of_difference in Hnin as [Hnin|Hnin].
+            + assert (ρ ∉ live_roles _ (trace_last auxtr)).
+              eapply not_elem_of_weaken => //.
+              { epose proof ls_fuel_dom. set_solver. }
+              assert (ρ ∈ dom fs2) by set_solver. set_solver.
+            + apply elem_of_difference in Hnin as [? Hnin].
+              apply not_elem_of_dom in Hnin. rewrite Hnin /= in Hlim.
+              by apply Hlim. }
+          split.
+          { intros ρ'. unfold update_fuel_resource, fuel_apply => Hin.
+            rewrite map_imap_dom_eq in Hin; last first.
+            { intros ρ0 _ Hin'. destruct (decide (ρ0 ∈ dom fs2)); [by apply elem_of_dom|].
+              rewrite dom_gset_to_gmap elem_of_difference in Hin'.
+              destruct Hin' as [Hin' ?]. apply elem_of_union in Hin' as [?|?]; [by apply elem_of_dom|done]. }
+            rewrite dom_gset_to_gmap in Hin. rewrite map_lookup_imap lookup_gset_to_gmap option_guard_True /=; last set_solver.
+            assert (ρ' ∈ dom fs2) by set_solver. rewrite decide_True //. apply Hnewlim. apply elem_of_difference; split =>//.
+            intros contra%Hxdom%elem_of_dom_2. rewrite ls_same_doms in contra. simplify_eq. set_solver. }
+          intros ρ0 Hin.
+          assert (ρ0 ∉ live_roles _ (trace_last auxtr)).
+          { eapply not_elem_of_weaken; last apply ls_fuel_dom. set_solver. }
+          apply elem_of_difference in Hin as [Hin1 Hnin].
+          assert (ρ0 ∈ live_roles _ s2).
+          { by_contradiction.
+            assert (ρ0 ∈ dom fs2).
+            { unfold update_fuel_resource, fuel_apply in Hin1.
+              eapply elem_of_subseteq in Hin1; last apply map_imap_dom_inclusion.
+              rewrite dom_gset_to_gmap in Hin1. set_solver. }
+            exfalso. assert (Hinabs: ρ0 ∈ dom fs1) by set_solver.
+            apply not_elem_of_dom in Hnin. rewrite Hauxtrlast Hfuel // in Hnin.
+            apply elem_of_dom in Hinabs. rewrite Hnin in Hinabs. simpl in Hinabs.
+            by inversion Hinabs. }
+          set_solver.
       - simplify_eq. unfold tids_smaller; simpl.
         intros ρ' ? Hmim.
-        rewrite map_lookup_imap in Hmim.
-        destruct (decide (ρ' ∈ live_roles _ s2)).
-        + rewrite lookup_gset_to_gmap option_guard_True //= in Hmim.
-          destruct (ls_mapping (trace_last auxtr) !! ρ') eqn:Heq.
-          * simpl in H. destruct (decide (ρ' ∈ live_roles _ (trace_last auxtr))) as [|Hnotin].
-            ** rewrite decide_True // in Hmim.
-               inversion Hstep; simplify_eq.
-               eapply from_locale_step =>//. by eapply Hless.
-            ** rewrite <- ls_mapping_dom in Hnotin. apply not_elem_of_dom in Hnotin. congruence.
-          * simpl in H. destruct (decide (ρ' ∈ live_roles _ (trace_last auxtr))) as [|Hnotin].
-            ** rewrite decide_True // in Hmim.
-               inversion Hstep; simplify_eq. eapply from_locale_step =>//.
-               by eapply Hless.
-            ** rewrite decide_False // in Hmim. simplify_eq.
-               inversion Hstep; simplify_eq. eapply from_locale_step =>//.
-               eapply Hless. eapply Hxdom. set_solver.
-        + rewrite lookup_gset_to_gmap option_guard_False //= in Hmim. }
+        rewrite map_lookup_imap in Hmim. rewrite lookup_gset_to_gmap in Hmim.
+        destruct (decide (ρ' ∈ (dom (ls_fuel (trace_last auxtr)) ∪ dom fs2) ∖ (dom fs1 ∖ dom fs2)));
+          last by rewrite option_guard_False in Hmim.
+        rewrite option_guard_True //= in Hmim.
+        destruct (decide (ρ' ∈ dom (ls_fuel (trace_last auxtr)))).
+        + rewrite decide_True // in Hmim.
+          inversion Hstep; simplify_eq.
+          eapply from_locale_step =>//. by eapply Hless.
+        + rewrite decide_False // in Hmim. simplify_eq.
+          inversion Hstep; simplify_eq.
+          eapply from_locale_step =>//. unfold from_locale. rewrite from_locale_from_Some //.
+          apply prefixes_from_spec. exists t1, t2. by list_simplifier. }
 
-    iFrame "Hfuel Hmod". iExists _. iFrame.
-    iSplitL "Hafuel".
-    { simpl. unfold update_fuel_resource.
-      destruct Hfuelsval as (?&?&?&?&Hdomeq).
-      iApply (own_proper with "Hafuel"). do 3 f_equiv.
-      rewrite !ls_fuel_dom !Hdomeq !Heq.
-      assert (live_roles _ s1 ∖ dom fs1 = live_roles _ s2 ∖ dom fs2).
-      { rewrite Hdomeq -leibniz_equiv_iff.
-        eapply set_subseteq_antisymm.
-        - intros ρ' [Hin Hnotin]%elem_of_difference.
-          apply elem_of_difference. split; last set_solver.
-          eapply fm_live_preserved; eauto. set_solver.
-        - intros ρ' [Hin Hnotin]%elem_of_difference. apply elem_of_difference.
-          split; [set_solver | set_solver]. }
-      rewrite -leibniz_equiv_iff.
-      eapply set_subseteq_antisymm; first set_solver.
-      intros ρ' Hin. apply elem_of_difference; split; [| set_solver].
-      apply elem_of_union.
-      destruct (decide (ρ' ∈ live_roles _ s1)); set_solver. }
-    iPureIntro. split; last first.
-    { intros ζ' ?. pose proof (locales_of_list_step_incl _ _ _ _ _ Hstep).
+    iFrame "Hfuel Hmod Hfr2". iExists _, _. iFrame. all: eauto. (* TODO: find source... *)
+    iPureIntro; split.
+
+    { intros ρ' ζ'. simpl. rewrite map_lookup_imap.
+      rewrite lookup_gset_to_gmap //=.
+      destruct (decide (ρ' ∈ (dom (ls_fuel δ1) ∪ dom fs2) ∖ (dom fs1 ∖ dom fs2))) as [Hin|Hnotin].
+      - rewrite option_guard_True //=. destruct (decide (ρ' ∈ dom (ls_fuel δ1))).
+        + destruct (decide (ζ' = ζ)) as [->|Hneq].
+          * rewrite lookup_insert. split.
+            { eexists; split =>//. apply elem_of_difference in Hin as [? Hin].
+              apply not_elem_of_difference in Hin as [?|?]; [|done].
+              set_solver. }
+            { intros (?&?&?). simplify_eq. apply Hxdom.
+              destruct Hfuelsval as (?&?&?&?&?). by_contradiction.
+              assert (ρ' ∈ live_roles Mdl s2 ∖ live_roles Mdl (trace_last auxtr)) by set_solver.
+              assert (ρ' ∈ fr1) by set_solver.
+              assert (ρ' ∈ FR) by set_solver.
+              assert (ρ' ∉ dom $ ls_fuel (trace_last auxtr)) by set_solver.
+              done. }
+          * rewrite lookup_insert_ne //.
+        + split.
+          * intros Htid. simplify_eq. rewrite lookup_insert. eexists; split=>//.
+            set_solver.
+          * assert (ρ' ∈ dom fs2) by set_solver. intros Hm. by_contradiction.
+            rewrite lookup_insert_ne in Hm; last congruence.
+            rewrite -Hinv in Hm. apply elem_of_dom_2 in Hm. rewrite ls_same_doms // in Hm.
+      - destruct Hfuelsval as (?&?&?&?&Hinf&?). rewrite option_guard_False //=. split; first done.
+        destruct (decide (ζ' = ζ)) as [->|Hneq].
+        { rewrite lookup_insert //. intros (?&?&?). simplify_eq. set_solver. }
+        rewrite lookup_insert_ne //.
+        rewrite -Hinv. intros Habs.
+
+        apply not_elem_of_difference in Hnotin as [Hnin|Hin].
+        + apply elem_of_dom_2 in Habs. rewrite ls_same_doms in Habs. set_solver.
+        + apply elem_of_difference in Hin as [Hin Hnin].
+          apply Hxdom in Hin. congruence. }
+    split.
+    { intros ζ' ?. pose proof (locales_of_list_step_incl _ _ _ _ _ Hstep). simpl.
       rewrite lookup_insert_ne; first by apply Hsmall; set_solver.
-      intros <-. destruct Hfuelsval as (_&Hfs1&_).
+      intros <-. destruct Hfuelsval as (_&_&Hfs1&_).
       rewrite <-Hxdom in Hfs1. apply Hinv in Hfs1 as (?&HM&?).
       rewrite Hsmall // in HM. set_solver. }
-
-    intros ρ' ζ'. simpl. rewrite map_lookup_imap.
-    destruct (decide (ρ' ∈ live_roles _ s2)) as [Hin|Hnotin].
-    - rewrite lookup_gset_to_gmap option_guard_True //=.
-      destruct (decide (ρ' ∈ live_roles _ δ1)) as [Hlive|Hlive].
-      + destruct (decide (ζ = ζ')) as [<-|Hneq]; last by rewrite lookup_insert_ne //.
-        rewrite lookup_insert. split.
-        * rewrite Hinv. intros (ks&HM&Hks). eexists. split; first done.
-          destruct Hfuelsval as (?&?&?&?&->). apply elem_of_union.
-          left. apply elem_of_intersection. split; last done. apply Hxdom.
-          apply Hinv. eexists; split; done.
-        * intros (ks&HM&Hks). simplify_eq. apply Hxdom.
-          destruct Hfuelsval as (?&?&?&?&Hdomeq). rewrite Hdomeq in Hks.
-          set_solver.
-      + split.
-        * intros ?. simplify_eq. rewrite lookup_insert. eexists; split; first done.
-          destruct Hfuelsval as (?&?&?&?&->). set_solver.
-        * intros (ks&HM&Hks). simplify_eq.
-          destruct Hfuelsval as (?&?&?&?&Hdomeq).
-          assert (ζ = ζ'); last congruence.
-          destruct (decide (ζ = ζ')) as [|Hneq]; first done. exfalso.
-          rewrite lookup_insert_ne // in HM. unfold maps_inverse_match in Hinv.
-          assert (ls_mapping (trace_last auxtr) !! ρ' = Some ζ').
-          { apply Hinv. eexists; done. }
-          rewrite -ls_mapping_dom in Hlive. apply not_elem_of_dom in Hlive. set_solver.
-    - rewrite lookup_gset_to_gmap option_guard_False //=. split; first done.
-      intros (ks & HM & Hks). exfalso.
-      destruct (decide (ζ = ζ')) as [Heq'|Heq'].
-      + subst ζ'. rewrite lookup_insert in HM. simplify_eq.
-        destruct Hfuelsval as (_&_&_&_&Hdomeq). rewrite Hdomeq in Hks.
-        set_solver.
-      + rewrite lookup_insert_ne // in HM. unfold maps_inverse_match in Hinv.
-        assert (ls_mapping δ1 !! ρ' = Some ζ').
-        { apply Hinv. eexists _; eauto. }
-        eapply Hnotin, fm_live_preserved; eauto.
-        * rewrite -Heq -ls_mapping_dom. apply elem_of_dom. eauto.
-        * intros <-. destruct Hfuelsval as (?&?&?&?&_). set_solver.
-  Qed.
+    { simpl. rewrite /update_fuel_resource /fuel_apply.
+      rewrite map_imap_dom_eq ?dom_gset_to_gmap.
+      + apply elem_of_equiv_empty_L. intros ρ' [Hin1 Hin2]%elem_of_intersection.
+        apply elem_of_difference in Hin1 as [Hin11 Hin12].
+        apply not_elem_of_difference in Hin12.
+        apply elem_of_difference in Hin2 as [Hin21 Hin22].
+        apply not_elem_of_difference in Hin22.
+        assert (ρ' ∉ dom $ ls_fuel δ1) by set_solver.
+        assert (ρ' ∈ dom fs2) by set_solver.
+        destruct Hin12 as [Hin12|Hin12]; last by (epose proof ls_fuel_dom; set_solver).
+        destruct Hfuelsval as (?&?&?&?&?&?).
+        assert (ρ' ∉ dom fs1); last set_solver.
+        intros contra. pose proof (Hfuel _ contra) as Habs. apply elem_of_dom in contra as [? contra].
+        rewrite contra in Habs. apply elem_of_dom_2 in Habs. done.
+    + intros ρ' _ Hin. destruct (decide (ρ' ∈ dom fs2)) as [Hin'|].
+      * apply elem_of_dom in Hin' as [? ->]. done.
+      * assert (ρ' ∈ dom (ls_fuel δ1)) as Hin' by set_solver. apply elem_of_dom in Hin' as [? ->]. done. }
+Qed.
 
 End model_state_lemmas.
