fairness/fairness_finiteness.v
@@ -1,4 +1,4 @@
-From trillium.fairness Require Import fairness resources.
+From trillium.fairness Require Import fairness.
 From trillium.prelude Require Import finitary quantifiers classical_instances.
 From stdpp Require Import finite.
 
@@ -42,8 +42,9 @@ Section finitary.
   Program Definition enumerate_next (δ1: (fair_model (Λ := Λ) M)) (oζ : olocale Λ) (c': cfg Λ):
     list (fair_model M * @mlabel (fair_model (Λ := Λ) M)) :=
     '(s2, ℓ) ← (δ1.(ls_under), None) :: enum_inner δ1.(ls_under);
-    fs ← enum_gmap_bounded' (live_roles _ s2) (max_gmap δ1.(ls_fuel) `max` fuel_limit s2);
-    ms ← enum_gmap_range_bounded' (live_roles _ s2) (locales_of_list c'.1);
+    d ← enumerate_dom_gsets' (dom δ1.(ls_fuel) ∪ live_roles _ s2);
+    fs ← enum_gmap_bounded' (live_roles _ s2 ∪ d) (max_gmap δ1.(ls_fuel) `max` fuel_limit s2);
+    ms ← enum_gmap_range_bounded' (live_roles _ s2 ∪ d) (locales_of_list c'.1);
     let ℓ' := match ℓ with
               | None => match oζ with
                          Some ζ => Silent_step ζ
@@ -58,10 +59,13 @@ Section finitary.
              ls_fuel := `fs;
              (* ls_fuel_dom := proj2_sig fs; *) (* TODO: why this does not work?*)
              ls_mapping := `ms ;
-             ls_mapping_dom := proj2_sig ms
           |}, ℓ').
   Next Obligation.
-    intros ??????????. destruct fs as [??]. by simpl.
+    intros ??????????. destruct fs as [? Heq]. rewrite /= Heq //. set_solver.
+  Qed.
+  Next Obligation.
+    intros ??????????. destruct fs as [? Heq]. destruct ms as [? Heq'].
+    rewrite /= Heq //.
   Qed.
 
   Lemma valid_state_evolution_finitary_fairness (φ: execution_trace Λ -> auxiliary_trace (fair_model M) -> Prop) :
@@ -76,43 +80,60 @@ Section finitary.
     split; last first.
     { destruct ℓ as [ρ tid' | |].
       - inversion Htrans as [Htrans']. apply elem_of_cons; right. by apply enum_inner_spec.
-      - apply elem_of_cons; left. f_equal. inversion Htrans as (?&?&?&?); done.
+      - apply elem_of_cons; left. f_equal. inversion Htrans as (?&?&?&?&?); done.
       - apply elem_of_cons; right. inversion Htrans as (?&?). by apply enum_inner_spec. }
-    apply elem_of_list_bind. eexists (δ2.(ls_fuel) ↾ (ls_fuel_dom _)); split; last first.
-    { eapply enum_gmap_bounded'_spec; split; first by apply ls_fuel_dom.
+    apply elem_of_list_bind. eexists (dom $ δ2.(ls_fuel)). split; last first.
+    { apply enumerate_dom_gsets'_spec. destruct ℓ as [ρ tid' | |].
+      - inversion Htrans as (?&?&?&?&?&?&?). intros ρ' Hin. destruct (decide (ρ' ∈ live_roles _ δ2)); first set_solver.
+        destruct (decide (ρ' ∈ dom $ ls_fuel (trace_last auxtr))); first set_solver. set_solver.
+      - inversion Htrans as (?&?&?&?&?). set_solver.
+      - inversion Htrans as (?&?&?&?&?). done. }
+    apply elem_of_list_bind.
+    assert (Hfueldom: dom δ2.(ls_fuel) = live_roles M δ2 ∪ dom (ls_fuel δ2)).
+    { rewrite subseteq_union_1_L //. apply ls_fuel_dom. }
+
+    eexists (δ2.(ls_fuel) ↾ Hfueldom); split; last first.
+    { eapply enum_gmap_bounded'_spec; split =>//.
       intros ρ f Hsome. destruct ℓ as [ρ' tid' | |].
       - destruct (decide (ρ = ρ')) as [-> | Hneq].
-        + inversion Htrans as [? Hbig]. destruct Hbig as (?&?&?&Hlim&?).
-          rewrite Hsome /= in Hlim.
-          assert (Hlive: ρ' ∈ live_roles _ δ2).
-          { rewrite -ls_fuel_dom elem_of_dom. eauto. }
-          specialize (Hlim Hlive). lia.
-        + inversion Htrans as [? Hbig]. destruct Hbig as (?&?&Hleq&?&Hnew).
-          destruct (decide (ρ ∈ live_roles _ (trace_last auxtr))) as [Hin|Hnotin].
+        + inversion Htrans as [? Hbig]. destruct Hbig as (Hmap&Hleq&?&Hlim&?&?).
+          destruct (decide (ρ' ∈ live_roles _ δ2)).
+          * rewrite Hsome /= in Hlim.
+            assert (Hlive: ρ' ∈ live_roles _ δ2) by set_solver.
+            specialize (Hlim Hlive). lia.
+          * unfold fuel_decr in Hleq.
+            apply elem_of_dom_2 in Hmap. rewrite ls_same_doms in Hmap.
+            pose proof Hsome as Hsome'. apply elem_of_dom_2 in Hsome'.
+            specialize (Hleq ρ' ltac:(done) ltac:(done)).
+            assert(must_decrease ρ' (Some ρ') (trace_last auxtr) δ2 (Some tid')) as Hmd; first by constructor 3.
+            specialize (Hleq Hmd). rewrite Hsome /= in Hleq.
+            apply elem_of_dom in Hmap as [? Heq]. rewrite Heq in Hleq.
+            pose proof (max_gmap_spec _ _ _ Heq). simpl in *. lia.
+        + inversion Htrans as [? Hbig]. destruct Hbig as (Hmap&?&Hleq'&?&Hnew&?).
+          destruct (decide (ρ ∈ dom $ ls_fuel (trace_last auxtr))) as [Hin|Hnotin].
           * assert (Hok: oleq (ls_fuel δ2 !! ρ) (ls_fuel (trace_last auxtr) !! ρ)).
-            { apply Hleq =>//. congruence. }
+            { unfold fuel_must_not_incr in *.
+              assert (ρ ∈ dom $ ls_fuel (trace_last auxtr)) by SS.
+              specialize (Hleq' ρ ltac:(done) ltac:(congruence)) as [Hleq'|Hleq'] =>//. apply elem_of_dom_2 in Hsome. set_solver. }
             rewrite Hsome in Hok. destruct (ls_fuel (trace_last auxtr) !! ρ) as [f'|] eqn:Heqn; last done.
-            rewrite <-ls_fuel_dom, elem_of_dom in Hin.
             pose proof (max_gmap_spec _ _ _ Heqn). simpl in *. lia.
           * assert (Hok: oleq (ls_fuel δ2 !! ρ) (Some (fuel_limit δ2))).
-            { apply Hnew. apply elem_of_dom_2 in Hsome. rewrite -ls_fuel_dom. set_solver. }
-            rewrite Hsome in Hok. simpl in *. lia.
-      - inversion Htrans as [? [? [Hleq Heq]]]. specialize (Hleq ρ).
-        assert (Hok: oleq (ls_fuel δ2 !! ρ) (ls_fuel (trace_last auxtr) !! ρ)).
-        { apply Hleq; last done. rewrite Heq -ls_fuel_dom elem_of_dom Hsome. by eauto. }
-        rewrite Hsome in Hok. destruct (ls_fuel (trace_last auxtr) !! ρ) as [f'|] eqn:Heqn; last done.
-        pose proof (max_gmap_spec _ _ _ Heqn). simpl in *. lia.
-      - inversion Htrans as [? [? [Hleq Hnew]]]. specialize (Hleq ρ).
-        destruct (decide (ρ ∈ live_roles _ (trace_last auxtr))).
-        + assert (Hok: oleq (ls_fuel δ2 !! ρ) (ls_fuel (trace_last auxtr) !! ρ)).
-          { apply Hleq; done. }
-          rewrite Hsome in Hok. destruct (ls_fuel (trace_last auxtr) !! ρ) as [f'|] eqn:Heqn; last done.
+            { apply Hnew. apply elem_of_dom_2 in Hsome. set_solver. }
+            rewrite Hsome in Hok. simpl in Hok. lia.
+      - inversion Htrans as [? [? [Hleq [Hincl Heq]]]]. specialize (Hleq ρ).
+        assert (ρ ∈ dom $ ls_fuel (trace_last auxtr)) as Hin.
+        { apply elem_of_dom_2 in Hsome. set_solver. }
+        specialize (Hleq Hin ltac:(done)) as [Hleq|Hleq].
+        + rewrite Hsome in Hleq. destruct (ls_fuel (trace_last auxtr) !! ρ) as [f'|] eqn:Heqn; last done.
           pose proof (max_gmap_spec _ _ _ Heqn). simpl in *. lia.
-        + assert (Hok: oleq (ls_fuel δ2 !! ρ) (Some (fuel_limit δ2))).
-          { apply Hnew. apply elem_of_dom_2 in Hsome. rewrite -ls_fuel_dom. set_solver. }
-          rewrite Hsome in Hok. simpl in *. lia. }
-    apply elem_of_list_bind. exists (δ2.(ls_mapping) ↾ (ls_mapping_dom _)); split; last first.
-    { eapply enum_gmap_range_bounded'_spec; split; first by apply ls_mapping_dom.
+        + apply elem_of_dom_2 in Hsome. set_solver.
+      - inversion Htrans as [? [? [Hleq [Hnew Hfalse]]]]. done. }
+    apply elem_of_list_bind.
+    assert (Hmappingdom: dom δ2.(ls_mapping) = live_roles M δ2 ∪ dom (ls_fuel δ2)).
+    { rewrite -Hfueldom ls_same_doms //. }
+
+    exists (δ2.(ls_mapping) ↾ Hmappingdom); split; last first.
+    { eapply enum_gmap_range_bounded'_spec; split=>//.
       intros ρ' tid' Hsome. unfold tids_smaller in *.
       apply locales_of_list_from_locale_from. eauto. }
     rewrite elem_of_list_singleton; f_equal.
@@ -121,5 +142,7 @@ Section finitary.
       Unshelve.
       + intros ??. apply make_decision.
       + intros. apply make_proof_irrel.
+      + done.
+      + done.
   Qed.
 End finitary.
